Refactor compiler (less non-extracted code).

extraction/lvcc.ml
@@ -16,45 +16,21 @@ let main () =
     ("-o",Arg.Set_string outfile, "Place the output into <file>");
     ("-O", Arg.Bool set_optimize, "Enable optimization (default is on)")
   ] in
+  let print_string a s = Printf.eprintf "%s" (implode s); a in
+  let toString_nstmt s = explode (print_nexpr 0 s !ids) in
+  let toString_stmt s = explode (print_expr 0 s !ids) in
+  let toString_ann s p a = explode (print_ann (fun s -> implode (p s)) 0 a) in
+  let toString_set s = explode (print_set !ids s) in
+  let toString_list s = explode (print_list (fun x -> print_var x !ids) "," s) in
     Arg.parse speclist set_infile ("usage: lvc [options]");
     try
       let file_chan = open_in !infile in
       let lexbuf = Lexing.from_channel  file_chan in
-      let result = Parser.expr Lexer.token lexbuf in
-      let _ = Printf.printf "Normalized Input:\n%s\n\n" (print_nexpr 0 result !ids) in
-      match (Lvc.labIndices result []) with
-        | Lvc.Error s -> let _ = Printf.printf "Ill-formed program (probably undeclared
-          function)" in ()
-        | Lvc.Success ili -> 
-          let lv = Lvc.livenessAnalysis generic_first ili in
-          let _ = Printf.printf "Liveness\n%s\n\n" (print_ann (print_set !ids) 0 lv) in
-          let aa = Lvc.additionalArguments ili lv in
-          let _ = Printf.printf "AdditionalArguments\n%s\n\n" 
-	    (print_ann (print_list (fun s -> "[" ^ (print_var s !ids) ^ "]") " ") 0 aa) in
-          let v = Lvc.toILF result lv in
-          let _ = match v with 
-	    | Lvc.Success ilf -> Printf.printf "toILF compilate:\n%s\n\n" (print_expr 0 ilf !ids);
-	      let copyProp = Lvc.copyPropagate (fun x -> x) ilf in
-	      let _ = Printf.printf "Copy Propagated\n%s\n\n" (print_expr 0 copyProp !ids) in	  
-
-	      let ren = Lvc.rename_apart copyProp in
-              let _ = Printf.printf "Renamed apart\n%s\n\n" (print_expr 0 ren (BigMap.empty)) in
-	      let lv2 = Lvc.livenessAnalysis generic_first ren in
-              let _ = Printf.printf "Liveness\n%s\n\n" (print_ann (print_set BigMap.empty) 0 lv2) in
-	      (match (Lvc.linear_scan ren lv2 (fun x -> x)) with
-		| Lvc.Success renaming -> 
-		  let alloc = Lvc.rename renaming ren in
-		  let _ = Printf.printf "Allocated\n%s\n\n" (print_expr 0 alloc (BigMap.empty)) in
-(*		  let lv3 = Lvc.live_rename renaming lv2 in
-		  let _ = Printf.printf "Liveness\n%s\n\n" (print_ann (print_set (BigMap.empty)) 0 lv3) in*)
-		  (let v = Lvc.fromILF Lvc.linear_scan parallel_move generic_first copyProp in
-		   match v with
-		     | Lvc.Success s -> Printf.printf "Compilate:\n%s\n\n" 
-		       (print_expr 0 s (BigMap.empty));
-                     | Lvc.Error e -> Printf.printf "Compilation failed:%s\n\n" (implode e) )
-                | Lvc.Error e -> Printf.printf "Compilation failed:\n%s" (implode e))
-            | Lvc.Error e -> Printf.printf "Compilation failed:\n%s" (implode e) in
-          ()
+      let ilin = Parser.expr Lexer.token lexbuf in
+      match Lvc.toILF generic_first print_string toString_nstmt toString_stmt toString_ann toString_set toString_list ilin 0 with
+      | (Lvc.Success ilf, _) -> 
+	 Printf.printf "toILF compilate:\n%s\n\n" (print_expr 0 ilf !ids);
+      | (Lvc.Error e, _) -> Printf.printf "Compilation failed:\n%s" (implode e);
     with Parsing.Parse_error ->
         Printf.eprintf "A parsing error occured \n"
       | Sys_error s-> Printf.eprintf "%s\n" s
