extraction/util.ml
@@ -9,8 +9,15 @@ let implode l =
   let res = String.create (List.length l) in
   let rec imp i = function
     | [] -> res
-    | c :: l -> res.[i] <- c; imp (i + 1) l in
-    imp 0 l
+    | '\\' :: 'n' :: l -> res.[i] <- '\n'; imp (i + 2) l
+    | c :: l -> res.[i] <- c; imp (i + 1) l 
+    in imp 0 l
+
+
+let explode s =
+  let rec exp i l =
+    if i < 0 then l else exp (i - 1) (s.[i] :: l) in
+  exp (String.length s - 1) []
 
 let rec discard_dead lv m =
   match lv, m with
