Compiler.v
@@ -1,11 +1,11 @@
 Require Import List CSet.
 Require Import Util AllInRel IL ILRaise EnvTy ParamsMatch RegAlloc RenameApart Sim Status.
-Require Coherence ILIToILF Liveness ParallelMove ILN LivenessAnalysis CoherenceAlgo RegAllocAlgo CopyPropagation.
+Require Coherence ILIToILF Liveness ParallelMove ILN LivenessAnalysis CoherenceAlgo RegAllocAlgo CopyPropagation DVE.
 
 Require Import ExtrOcamlBasic.
 Require Import ExtrOcamlZBigInt.
 Require Import ExtrOcamlNatBigInt.
-Require Import ExtrOcamlString.
+Require Import String ExtrOcamlString.
 
 Set Implicit Arguments.
 
@@ -16,23 +16,59 @@ Hypothesis ssa_construction : stmt -> ann (option (set var)) * ann (list var).
 Hypothesis parallel_move : var -> list var -> list var -> (list(list var * list var)).
 Hypothesis first : ann (set var) -> ( ann (set var) -> ann (set var) * bool) -> ann (set var).
 
+
 Definition livenessAnalysis (s:stmt) :=
 @AbsInt.analysis (set var) Subset (@Subset_computable _ _ ) first _ _ _ LivenessAnalysis.liveness_analysis s.
 
 Definition additionalArguments s lv :=
   fst (CoherenceAlgo.computeParameters nil nil nil s lv).
 
-Definition toILF (ilin:ILN.nstmt) (lv:ann (set var)) : status IL.stmt :=
-  sdo ili <- ILN.labIndices ilin nil; 
-  if [Liveness.live_sound nil ili lv] then
-    let additional_arguments := additionalArguments ili lv
-    in if [ILIToILF.trs nil nil ili lv additional_arguments] then
-         Success (ILIToILF.compile nil ili additional_arguments)
-       else Error ("Additional Arguments insufficient")
-    else Error ("Liveness unsound").
+Class ToString (T:Type) := toString : T -> string.
 
-Definition optimize (s:stmt) : stmt := CopyPropagation.copyPropagate id s.
+Hypothesis Dummy : Type.
+Hypothesis print_string : Dummy -> string -> Dummy.
 
+Hypothesis toString_nstmt : ILN.nstmt -> string.
+Instance ToString_nstmt : ToString ILN.nstmt := toString_nstmt.
+
+Hypothesis toString_stmt : stmt -> string.
+Instance ToString_stmt : ToString stmt := toString_stmt.
+
+Hypothesis toString_ann : forall A, (A -> string) -> ann A -> string.
+Instance ToString_ann {A} `{ToString A} : ToString (ann A) := 
+  toString_ann (@toString A _).
+
+Hypothesis toString_live : set var -> string. 
+Instance ToString_live : ToString (set var) := toString_live.
+
+Hypothesis toString_list : list var -> string. 
+Instance ToString_list : ToString (list var) := toString_list.
+
+Notation "'///' S '///' x '///' y ';' s" := (let S := print_string S (x ++ "\n" ++ toString y ++ "\n\n") in s) (at level 200).
+
+Notation "'ensure' x 'by' y 'fail' S ; s" := 
+  (if [ y ] then s else (Error ("Error: " ++ x),S)) (at level 200).
+
+Definition toILF (ilin:ILN.nstmt) (S:Dummy) : status IL.stmt * Dummy :=
+  /// S /// "Input " /// ilin ;
+  match ILN.labIndices ilin nil with
+    | Success ili => 
+      /// S /// "Normalized Input " /// ili ;
+        let lv := livenessAnalysis ili in
+        /// S /// "Liveness Information " /// lv ; 
+        ensure "Liveness information sound" by Liveness.true_live_sound nil ili lv fail S;
+          let ilid := DVE.compile ili lv in
+          /// S /// "DVE" /// ilid ; 
+          let additional_params := additionalArguments ilid lv in
+          /// S /// "Additional Params" /// additional_params ; 
+          ensure "Additional parameters sufficient" 
+            by ILIToILF.trs nil nil ili (DVE.compile_live ili lv) additional_params fail S;
+            (Success (ILIToILF.compile nil ilid additional_params), S)
+    | x => (x,S)
+  end.
+
+Definition optimize (s:stmt) : stmt := 
+  CopyPropagation.copyPropagate id s.
 
 Definition fromILF (s:stmt) : status stmt :=
   let s_renamed_apart := rename_apart s
@@ -49,14 +85,16 @@ Definition fromILF (s:stmt) : status stmt :=
          Error "Register allocation not injective."
      else
        Error "Liveness unsound.".
-Lemma toILF_correct ilin alv s (E:env val)
-  : toILF ilin alv = Success s
+
+Opaque Liveness.live_sound_dec.
+Opaque ILIToILF.trs_dec.
+(*
+Lemma toILF_correct ilin alv s (E:env val) e
+  : toILF ilin alv = (Success s, e)
    -> @sim _ ILN.statetype_I _ _ (ILN.I.labenv_empty, E, ilin) 
           (nil:list F.block, E, s).
 Proof.
-  intros. unfold toILF in H; simpl in *.
-  Opaque Liveness.live_sound_dec.
-  Opaque ILIToILF.trs_dec.
+  intros. unfold toILF in H. simpl in *.
   monadS_inv H.
   destruct if in EQ0.
   destruct if in EQ0; isabsurd. inv EQ0.
@@ -64,7 +102,7 @@ Proof.
   econstructor; eauto; isabsurd. econstructor; isabsurd.
   econstructor; eauto using AIR4; eauto; try reflexivity; isabsurd.
 
-  econstructor; eauto 30 using ILIToILF.compile_typed, agree_on_refl, AIR2, PIR2; isabsurd.
+  econstructor; eauto 30 using ILIToILF.compile_typed, agree_on_refl, AIR2, PIR2; isabsurd. 
   eapply (@ILIToILF.live_sound_compile nil); eauto.
   isabsurd.
 Qed.
@@ -104,24 +142,27 @@ Proof.
   congruence.
 Qed.
 
-Lemma optimize_correct E s
- : sim (nil:list F.block, E, s) (nil:list F.block, E, optimize s).
+Lemma optimize_correct E s lv
+ : sim (nil:list F.block, E, s) (nil:list F.block, E, optimize s lv).
 Proof.
   unfold optimize.
+  eapply (@sim_trans F.state _ F.state _). 
+  instantiate (1:= (nil, E, DVE.compile s lv)).
+  admit.
   eapply (@sim_trans F.state _ F.state _). 
   eapply CopyPropagation.subst_id.
   eapply sim_sym.
   eapply CopyPropagation.sim_CP. 
 Qed.
-
+*)
 End Compiler.
 
-Print Assumptions toILF_correct. 
-Print Assumptions fromILF_correct.
+(*Print Assumptions toILF_correct. 
+Print Assumptions fromILF_correct.*)
  
-Extraction Inline bind Option.bind.
+Extraction Inline bind Option.bind toString.
 
-Extraction "extraction/lvc.ml" toILF fromILF RegAllocAlgo.linear_scan CopyPropagation.copyPropagate.
+Extraction "extraction/lvc.ml" toILF fromILF RegAllocAlgo.linear_scan optimize.
 
 
 
